upd

code/experimental/P256/Hacl.Spec.P256.Ladder.fst
@@ -5,6 +5,8 @@ open Lib.Buffer
 
 open Hacl.Spec.P256.Definitions
 open Hacl.Spec.P256.MontgomeryMultiplication
+open Hacl.Spec.P256.MontgomeryMultiplication.PointAdd 
+open Hacl.Spec.P256.MontgomeryMultiplication.PointDouble
 
 open FStar.Math.Lemmas
 open Lib.Sequence
@@ -16,3 +18,88 @@ type scalar = lbytes 32
 let ith_bit (k:scalar) (i:nat{i < 256}) : uint64 =
 	let q = i / 8 in let r = size (i % 8) in
  	to_u64 ((index k q >>. r) &. u8 1)
+
+let pr = p:lseq uint64 4 {let t = sub p 0 4 in  felem_seq_as_nat t < prime}
+
+assume val fromDomainPoint: tuple3 nat nat nat -> tuple3 nat nat nat
+assume val toDomainPoint: tuple3 nat nat nat -> tuple3 nat nat nat
+
+assume val point_add:  p: point_prime -> q: point_prime -> Tot (r: point_prime
+  {
+    let px, py, pz = felem_seq_as_nat(sub p 0 4), felem_seq_as_nat(sub p 4 4), felem_seq_as_nat(sub p 8 4) in 
+    let qx, qy, qz = felem_seq_as_nat(sub q 0 4), felem_seq_as_nat(sub q 4 4), felem_seq_as_nat(sub q 8 4) in 
+    let rx, ry, rz = felem_seq_as_nat(sub r 0 4), felem_seq_as_nat(sub r 4 4), felem_seq_as_nat(sub r 8 4) in 
+    
+    let pxD, pyD, pzD = fromDomainPoint (px, py, pz) in 
+    let qxD, qyD, qzD = fromDomainPoint (qx, qy, qz) in 
+    let rxD, ryD, rzD = fromDomainPoint (rx, ry, rz) in 
+ 
+    let x3N, y3N, z3N = _point_add (pxD, pyD, pzD) (qxD, qyD, qzD) in 
+    x3N == rxD /\ y3N == ryD /\ z3N == rzD
+  }
+)
+
+assume val point_double:  p: point_prime -> Tot (r: point_prime
+  {
+    let px, py, pz = felem_seq_as_nat(sub p 0 4), felem_seq_as_nat(sub p 4 4), felem_seq_as_nat(sub p 8 4) in 
+    let rx, ry, rz = felem_seq_as_nat(sub r 0 4), felem_seq_as_nat(sub r 4 4), felem_seq_as_nat(sub r 8 4) in 
+    
+    let pxD, pyD, pzD = fromDomainPoint (px, py, pz) in 
+    let rxD, ryD, rzD = fromDomainPoint (rx, ry, rz) in 
+ 
+    let x3N, y3N, z3N = _point_double (pxD, pyD, pzD) in
+    x3N == rxD /\ y3N == ryD /\ z3N == rzD
+  }
+)
+
+
+val _ml_step0: p: point_nat -> q: point_nat -> tuple2 point_nat point_nat
+
+let _ml_step0 r0 r1 = 
+  let r0 = _point_add r0 r1 in
+  let r1 = _point_double r1 in 
+  (r0, r1)
+
+val _ml_step1: p: point_prime -> q: point_prime -> tuple2 point_prime point_prime
+
+let _ml_step1 r0 r1 = 
+  let r3 = point_double r0 in 
+  let r1 = point_add r0 r1 in 
+  (r3, r1)
+
+
+assume val montgomery_ladder_step0: p: point_prime -> q: point_prime -> 
+  Tot (r: tuple2 point_prime point_prime 
+    {
+      let r0, r1 = r in 
+
+      let x3_0 = felem_seq_as_nat (sub r0 0 4) in 
+      let y3_0 = felem_seq_as_nat (sub r0 4 4) in
+      let z3_0 = felem_seq_as_nat (sub r0 8 4) in 
+
+      let x3_1 = felem_seq_as_nat (sub r1 0 4) in 
+      let y3_1 = felem_seq_as_nat (sub r1 4 4) in 
+      let z3_1 = felem_seq_as_nat (sub r1 8 4) in 
+    
+      let x1 = felem_seq_as_nat (sub p 0 4) in 
+      let y1 = felem_seq_as_nat (sub p 4 4) in 
+      let z1 = felem_seq_as_nat (sub p 8 4) in 
+      
+      let x2 = felem_seq_as_nat (sub q 0 4) in 
+      let y2 = felem_seq_as_nat (sub q 4 4) in 
+      let z2 = felem_seq_as_nat (sub q 8 4) in
+    
+      let pxD, pyD, pzD = fromDomainPoint (x1, y1, z1) in 
+      let qxD, qyD, qzD = fromDomainPoint (x2, y2, z2) in 
+      let x3D_0, y3D_0, z3D_0 = fromDomainPoint (x3_0, y3_0, z3_0) in
+      let x3D_1, y3D_1, z3D_1 = fromDomainPoint (x3_1, y3_1, z3_1) in 
+
+      let r0N, r1N = _ml_step0 (pxD, pyD, pzD) (qxD, qyD, qzD) in 
+      let (x3N_0, y3N_0, z3N_0) = r0N in 
+      let (x3N_1, y3N_1, z3N_1) = r1N in 
+    
+      x3N_0 == x3D_0 /\  y3N_0 == y3D_0 /\  z3N_0 == z3D_0 /\ 
+      x3N_1 == x3D_1 /\  y3N_1 == y3D_1 /\  z3N_1 == z3D_1 
+    }
+ )   
+    
